Complete most of `Sub_AndEqz_iff_eq_one` proof
Convert `RBMap`s into `List`s

Is0.lean
@@ -1,6 +1,7 @@
 import Mathlib.Data.Nat.Prime
 import Mathlib.Data.Vector
 import Mathlib.Data.ZMod.Defs
+import Mathlib.Data.ZMod.Basic
 
 @[inline]
 def P: ℕ := 15 * 2^27 + 1
@@ -16,18 +17,16 @@ inductive Lit where
   | Val : Felt → Lit
   | Constraint : Prop → Lit
 
--- A mapping of variable names to values.
---
--- Note: we can have duplicate keys if one maps to a felt and the other to a
--- constraint...
+-- A pair of append-only stacks of assignments. Basically, this is where we
+-- store the evaluated value of the expression on each line.
 structure State where
-  felts : Std.RBMap String Felt cmp
-  constraints : Std.RBMap String Prop cmp
+  felts : List Felt
+  constraints : List Prop
 
 -- A parametrized expression. In practice, α will be either `Felt` or `Prop`.
 inductive Expression (α : Type) where
   | Literal : α → Expression α
-  | Variable : String → Expression α
+  | Variable : ℕ → Expression α
 
 -- An operation from the cirgen (circuit generation) MLIR dialect.
 inductive Op where
@@ -41,7 +40,7 @@ inductive Op where
   | Inv : Felt → Op
   | AndEqz : Expression Prop → Expression Felt → Op
   | AndCond : Prop → Felt → Prop → Op
-  | Variable : String → Op
+  | Variable : ℕ → Op
 
 -- Evaluate a circuit operation to get some kind of literal.
 def Op.eval (state : State) (op : Op) : Lit :=
@@ -50,54 +49,58 @@ def Op.eval (state : State) (op : Op) : Lit :=
   | True => .Constraint (_root_.True)
   | Get buffer i _ => .Val (buffer.get i)
   | Sub x y => .Val (x - y)
-  | Variable name => .Val (state.felts.findD name 0)
+  | Variable i => .Val (state.felts.getD i 0)
   | AndEqz c x =>
-    match c with
-    | .Literal c => .Constraint (c ∧ x = .Literal 0)
-    | .Variable name =>  .Constraint ((state.constraints.findD name _root_.True) ∧ x = .Literal 0)
+    match c, x with
+    | .Literal c, .Literal x => .Constraint (c ∧ x = 0)
+    | .Literal c, .Variable j => .Constraint (c ∧ (state.felts.getD j 17) = 0)
+    | .Variable i, .Literal x =>  .Constraint ((state.constraints.getD i _root_.True) ∧ x = 0)
+    | .Variable i, .Variable j =>  .Constraint ((state.constraints.getD i _root_.True) ∧ (state.felts.getD j 17) = 0)
   | _ => .Constraint False
 
--- Evaluate `op` and assign its value to `name` in the `state` context.
-def Op.assign (state : State) (op : Op) (name : String) : State :=
+-- Evaluate `op` and push its literal value to the stack.
+def Op.assign (state : State) (op : Op) : State :=
   match (Op.eval state op) with
-  | .Val x => { state with felts := state.felts.insert name x }
-  | .Constraint c => { state with constraints := state.constraints.insert name c }
+  | .Val x => { state with felts := x :: state.felts }
+  | .Constraint c => { state with constraints := c :: state.constraints }
 
 -- An MLIR program in the `cirgen` (circuit generation) dialect.
 inductive Cirgen where
+  | Assign : Op → Cirgen
+  | Return : ℕ → Cirgen
   | Sequence : Cirgen → Cirgen → Cirgen
-  | Assign : String → Op → Cirgen
-  | Return : String → Cirgen
 
 -- Step through the entirety of a `Cirgen` MLIR program from initial state
 -- `state`, yielding the post-execution state and possibly a constraint
 -- (`Prop`).
 def Cirgen.step (state : State) (program : Cirgen) : State × Option Prop :=
   match program with
-  -- We may want to encode the index of the instruction in `State`, and then
-  -- always assign to the index instead of using a name.
-  | Assign name op => (Op.assign state op name, none)
+  | Assign op => (Op.assign state op, none)
   | Sequence a b => let (state', x) := Cirgen.step state a
                     match x with
                     | some x => (state', some x)
                     | none => Cirgen.step state' b
-  | Return name => (state, some $ state.constraints.findD name _root_.True)
+  | Return i => (state, some $ state.constraints.getD i _root_.True)
 
 -- The result of stepping through a program that generates `(1 - x) = 0`, which
 -- should be equivalent to checking `x = 1`.
 def subAndEqzActual (x : Felt) : State × Option Prop :=
-  Cirgen.step { felts := Std.RBMap.empty, constraints := Std.RBMap.empty }
+  Cirgen.step { felts := [], constraints := [] }
     (.Sequence
       (.Sequence
-        (.Assign "x-1" (Op.Sub x 1))
-        (.Assign "(x-1)=0"
-          (.AndEqz (.Literal _root_.True) (.Variable "x-1"))))
-      (.Return "(x-1)=0"))
+        (.Assign (Op.Sub x 1))
+        (.Assign (.AndEqz (.Literal _root_.True) (.Variable 0))))
+      (.Return 0))
+
+#eval (subAndEqzActual 1).1.1
+#eval (subAndEqzActual 0).1.1
+#eval (subAndEqzActual 2).1.1
+#eval (subAndEqzActual 1).1.2
 
 -- The expected post-execution state after computing `subAndEqzActual`.
 def subAndEqzExpectedState (x : Felt) : State :=
-  { felts := Std.RBMap.ofList [("x-1", x - 1)] cmp
-  , constraints := Std.RBMap.ofList [("(x-1)=0", x - 1 = (0 : Felt))] cmp
+  { felts := [x - 1]
+  , constraints := [x - 1 = 0]
   }
 
 -- Check that our `(1 - x) = 0` program is equivalent to `x = 1`.
@@ -106,7 +109,14 @@ theorem Sub_AndEqz_iff_eq_one :
     ∧ (((subAndEqzActual x).2 = some c) → (c ↔ x = 1)) := by
   intros x
   apply And.intro
-  sorry
+  unfold subAndEqzActual
+  unfold subAndEqzExpectedState
+  unfold Cirgen.step
+  unfold Cirgen.step
+  unfold Cirgen.step
+  unfold Op.assign
+  unfold Op.eval
+  simp only [List.getD_cons_zero, true_and]
   intros h
   unfold subAndEqzActual at h
   rw [Prod.snd] at h
@@ -122,3 +132,12 @@ theorem Sub_AndEqz_iff_eq_one :
   unfold Op.assign
   unfold Op.eval
   simp only [and_false]
+  simp only [List.getD_cons_zero, IsEmpty.forall_iff]
+  intros h
+  simp only [true_and] at h
+  sorry
+  intros h
+  rw [h]
+  unfold Op.assign
+  unfold Op.eval
+  simp only [List.getD_cons_zero]
